@prefix : <https://cogito.iot.linkeddata.es/def/iot#> .
@prefix sf: <http://www.opengis.net/ont/sf#> .
@prefix iot: <https://cogito.iot.linkeddata.es/def/iot#> .
@prefix owl: <http://www.w3.org/2002/07/owl#> .
@prefix rdf: <http://www.w3.org/1999/02/22-rdf-syntax-ns#> .
@prefix xml: <http://www.w3.org/XML/1998/namespace> .
@prefix xsd: <http://www.w3.org/2001/XMLSchema#> .
@prefix rdfs: <http://www.w3.org/2000/01/rdf-schema#> .
@prefix saref: <https://saref.etsi.org/core/> .
@prefix dcterms: <http://purl.org/dc/terms//> .
@prefix facility: <https://cogito.iot.linkeddata.es/def/facility#> .
@prefix resource: <https://cogito.iot.linkeddata.es/def/resource#> .
@base <https://cogito.iot.linkeddata.es/def/iot#> .

<https://cogito.iot.linkeddata.es/def/iot#> rdf:type owl:Ontology ;
                                             <http://purl.org/dc/elements/1.1/creator> "María Poveda Villalón" ,
                                                                                       "Raúl García Castro" ,
                                                                                       "Socorro  Bernardos Galindo" ;
                                             <http://purl.org/dc/elements/1.1/description> "The COGITO IoT ontology aims at modelling IoT devices and their measurements in the construction domain." ;
                                             <http://purl.org/dc/elements/1.1/title> "IoT ontology" ;
                                             <http://purl.org/dc/terms/license> <http://purl.org/NET/rdflicense/cc-by4.0> ;
                                             owl:versionInfo "0.5.0" .

#################################################################
#    Annotation properties
#################################################################

###  http://purl.org/dc/elements/1.1/creator
<http://purl.org/dc/elements/1.1/creator> rdf:type owl:AnnotationProperty .


###  http://purl.org/dc/elements/1.1/description
<http://purl.org/dc/elements/1.1/description> rdf:type owl:AnnotationProperty .


###  http://purl.org/dc/elements/1.1/title
<http://purl.org/dc/elements/1.1/title> rdf:type owl:AnnotationProperty .


###  http://purl.org/dc/terms/license
<http://purl.org/dc/terms/license> rdf:type owl:AnnotationProperty .


#################################################################
#    Object Properties
#################################################################

###  https://cogito.iot.linkeddata.es/def/iot#belongsToTagGroup
iot:belongsToTagGroup rdf:type owl:ObjectProperty ;
                      rdfs:range iot:TrackingTagGroup ;
                      rdfs:comment "Property relating an entity (especially an iot:TrackingTag) to an iot:TrackingTagGroup" ;
                      rdfs:label "belongs to tag group" .


###  https://cogito.iot.linkeddata.es/def/iot#hasLocation
iot:hasLocation rdf:type owl:ObjectProperty ;
                rdfs:comment "Property that relates an entity (especially a saref:Measurement) to the geo:Point it is located at" ;
                rdfs:label "has location" .


###  https://cogito.iot.linkeddata.es/def/iot#hasLocationKF
iot:hasLocationKF rdf:type owl:ObjectProperty ;
                  rdfs:comment "Property that relates an entity (especially a saref:Measurement) to the geo:Point it is located at using a KF transformation" ;
                  rdfs:label "has location KF" .


###  https://cogito.iot.linkeddata.es/def/iot#hasLocationMA
iot:hasLocationMA rdf:type owl:ObjectProperty ;
                  rdfs:comment "Property that relates an entity (especially a saref:Measurement) to the geo:Point it is located at using a MA transformation" ;
                  rdfs:label "has location MA" .


###  https://cogito.iot.linkeddata.es/def/iot#measuresLocation
iot:measuresLocation rdf:type owl:ObjectProperty ;
                     rdfs:subPropertyOf <https://saref.etsi.org/core#makesMeasurement> ;
                     rdfs:range iot:LocationMeasurement ;
                     rdfs:comment "Property relating an entity (especially an iot:TrackingTag) to an iot:LocationMeasurement" ;
                     rdfs:label "measures location" .


###  https://saref.etsi.org/core#isMeasurementOf
<https://saref.etsi.org/core#isMeasurementOf> rdf:type owl:ObjectProperty ;
                                              rdfs:isDefinedBy <https://saref.etsi.org/core#> ;
                                              rdfs:label "is measurement of" .


###  https://saref.etsi.org/core#makesMeasurement
<https://saref.etsi.org/core#makesMeasurement> rdf:type owl:ObjectProperty ;
                                               rdfs:isDefinedBy <https://saref.etsi.org/core#> ;
                                               rdfs:label "makes measurement" .


#################################################################
#    Data properties
#################################################################

###  http://purl.org/dc/terms/identifier
<http://purl.org/dc/terms/identifier> rdf:type owl:DatatypeProperty ;
                                      rdfs:isDefinedBy <http://purl.org/dc/terms/> ;
                                      rdfs:label "identifier" .


###  http://purl.org/dc/terms/titile
<http://purl.org/dc/terms/titile> rdf:type owl:DatatypeProperty ;
                                  rdfs:isDefinedBy <http://purl.org/dc/terms/> ;
                                  rdfs:label "title" .


###  https://cogito.iot.linkeddata.es/def/iot#coordX
iot:coordX rdf:type owl:DatatypeProperty ;
           rdfs:comment "Property referring to the coordinate x of a location measured by a tracking tag" ;
           rdfs:label "coordinate x" .


###  https://cogito.iot.linkeddata.es/def/iot#coordY
iot:coordY rdf:type owl:DatatypeProperty ;
           rdfs:comment "Property referring to the coordinate y of a location measured by a tracking tag" ;
           rdfs:label "coordinate y" .


###  https://cogito.iot.linkeddata.es/def/iot#coordZ
iot:coordZ rdf:type owl:DatatypeProperty ;
           rdfs:comment "Property referring to the coordinate z of a location measured by a tracking tag" ;
           rdfs:label "coordinate z" .


###  https://cogito.iot.linkeddata.es/def/iot#inferredAccuracy
iot:inferredAccuracy rdf:type owl:DatatypeProperty ;
                     rdfs:comment "Property referring to the accuracy of a location measured by  a tracking tag" ;
                     rdfs:label "inferred accuracy" .


###  https://cogito.iot.linkeddata.es/def/iot#inferredMovement
iot:inferredMovement rdf:type owl:DatatypeProperty ;
                     rdfs:comment "Property referring to the movement  associated to a location measured by a tracking tag" ;
                     rdfs:label "inferred movement" .


###  https://cogito.iot.linkeddata.es/def/iot#inferredSpeed
iot:inferredSpeed rdf:type owl:DatatypeProperty ;
                  rdfs:comment "Property referring to the speed  associated to a location measured by a tracking tag" ;
                  rdfs:label "inferred speed" .


###  https://cogito.iot.linkeddata.es/def/iot#locationRadius
iot:locationRadius rdf:type owl:DatatypeProperty ;
                   rdfs:comment "Property referring to the location radius associated to a location measured by a tracking tag" ;
                   rdfs:label "location radius" .


###  https://saref.etsi.org/core#hasTimestamp
<https://saref.etsi.org/core#hasTimestamp> rdf:type owl:DatatypeProperty ;
                                           rdfs:comment "has timestamp" ;
                                           rdfs:isDefinedBy <https://saref.etsi.org/core#> .


#################################################################
#    Classes
#################################################################

###  http://www.opengis.net/ont/sfl#Point
<http://www.opengis.net/ont/sfl#Point> rdf:type owl:Class ;
                                       rdfs:isDefinedBy <http://www.opengis.net/ont/geosparq#> ;
                                       rdfs:label "Point" .


###  https://cogito.iot.linkeddata.es/def/facility#SpatialZone
facility:SpatialZone rdf:type owl:Class ;
                     rdfs:comment "A subclass of bot:Zone and, as such, a part of the physical or a virtual world that is inherently both located in this world and has a 3D spatial extent." ;
                     rdfs:label "Spatial Zone" .


###  https://cogito.iot.linkeddata.es/def/iot#EquipmentTagGroup
iot:EquipmentTagGroup rdf:type owl:Class ;
                      rdfs:subClassOf iot:TrackingTagGroup ;
                      rdfs:comment "A tracking tag group belonging to a piece of equipment" ;
                      rdfs:label "Equipment Tag Group" .


###  https://cogito.iot.linkeddata.es/def/iot#HumanTagGroup
iot:HumanTagGroup rdf:type owl:Class ;
                  rdfs:subClassOf iot:TrackingTagGroup ;
                  rdfs:comment "A tracking tag group belonging to a human" ;
                  rdfs:label "Human Tag Group" .


###  https://cogito.iot.linkeddata.es/def/iot#LocationMeasurement
iot:LocationMeasurement rdf:type owl:Class ;
                        rdfs:subClassOf saref:Measurement ;
                        rdfs:comment "The location measured by an entity (especially an iot:TrackingTag)" ;
                        rdfs:label "Location Measurement" .


###  https://cogito.iot.linkeddata.es/def/iot#TrackedZone
iot:TrackedZone rdf:type owl:Class ;
                rdfs:subClassOf facility:SpatialZone ;
                rdfs:comment "An entity used to represent zones used by the IoT preprocessing module" ;
                rdfs:label "Tracked Zone" .


###  https://cogito.iot.linkeddata.es/def/iot#TrackingTag
iot:TrackingTag rdf:type owl:Class ;
                rdfs:subClassOf saref:Device ;
                rdfs:comment "A subclass of saref:Device and, as such, a tangible object designed to accomplish a particular task; in this case signalling its location" ,
                             "An entity" ;
                rdfs:label "Tracking Tag" .


###  https://cogito.iot.linkeddata.es/def/iot#TrackingTagGroup
iot:TrackingTagGroup rdf:type owl:Class ;
                     rdfs:comment "An entity used to group tracking tags" ;
                     rdfs:label "Tracking Tag Group" .


###  https://cogito.iot.linkeddata.es/def/resource#Resource
resource:Resource rdf:type owl:Class ;
                  rdfs:subClassOf saref:FeatureOfInterest ;
                  rdfs:comment "A source of supply, support, or aid, especially one that can be readily drawn upon when needed; and from which a property is measured" .


###  https://saref.etsi.org/core/Device
saref:Device rdf:type owl:Class ;
             rdfs:isDefinedBy <https://saref.etsi.org/core#> ;
             rdfs:label "Device" .


###  https://saref.etsi.org/core/FeatureOfInterest
saref:FeatureOfInterest rdf:type owl:Class ;
                        rdfs:isDefinedBy <https://saref.etsi.org/core#> ;
                        rdfs:label "Feature of Interest" .


###  https://saref.etsi.org/core/Measurement
saref:Measurement rdf:type owl:Class ;
                  rdfs:isDefinedBy <https://saref.etsi.org/core#> ;
                  rdfs:label "Measurement" .


###  Generated by the OWL API (version 4.5.9.2019-02-01T07:24:44Z) https://github.com/owlcs/owlapi
